exercises/ex_05_parallel_add_mul.v
@@ -58,12 +58,76 @@ Section proof.
   of [parallel_add_mul]. In this proof, you should use Boolean ghost variables,
   and the rules for those as given above. You are allowed to use any number of
   Boolean ghost variables. *)
+
+  (* ⌜⌝ *)
   Definition parallel_add_mul_inv (r : loc) (γ1 γ2 : gname) : iProp Σ :=
-    True%I. (* exercise: replace [True] with something meaningful. *)
+    (∃ b1 b2 : bool,
+        match b1, b2 with
+        | true, true => r ↦ #0
+        | false, true => r ↦ #2
+        | true, false => r ↦ #0
+        | false, false => bi_or (r ↦ #2) (r ↦ #4)
+        end
+          ∗ own γ1 (● (Excl' b1)) ∗ own γ2 (● (Excl' b2)))%I.
 
   Lemma parallel_add_mul_spec :
     {{{ True }}} parallel_add_mul {{{ z, RET #z; ⌜ z = 2 ∨ z = 4 ⌝ }}}.
   Proof.
     (* exercise *)
-  Admitted.
+    iIntros (Φ) "_ Post".
+    unfold parallel_add_mul. wp_alloc r as "Hr". wp_let.
+    iMod (ghost_var_alloc true) as (γ1) "[Hγ1● Hγ1◯]".
+    iMod (ghost_var_alloc true) as (γ2) "[Hγ2● Hγ2◯]".
+    wp_apply (newlock_spec (parallel_add_mul_inv r γ1 γ2) with "[Hr Hγ1● Hγ2●]").
+    { (* exercise *)
+      unfold parallel_add_mul_inv.
+      iExists true, true.
+      iFrame.
+    }
+    iIntros (l) "#Hl". wp_let.
+    (**********************************************)
+    (* ownership of ghost resources are splitted! *)
+    (**********************************************)
+    wp_apply (par_spec (λ _, own γ1 (◯ Excl' false)) (λ _, own γ2 (◯ Excl' false))
+                with "[Hγ1◯] [Hγ2◯]").
+    - wp_apply (acquire_spec with "Hl"). iDestruct 1 as (n1 n2) "(Hr & Hγ1● & Hγ2●)".
+      iDestruct (ghost_var_agree with "Hγ1● Hγ1◯") as %->.
+      iAssert (r ↦ #0)%I with "[Hr]" as "Hr".
+      { destruct n2; auto. }
+      wp_seq. wp_load. wp_op. wp_store.
+      iMod (ghost_var_update γ1 false with "Hγ1● Hγ1◯") as "[Hγ1● Hγ1◯]".
+      wp_apply (release_spec with "[- $Hl Hγ1◯]"); auto.
+      iExists _, _. iFrame "Hγ1● Hγ2●". destruct n2; auto.
+    - (* exercise *)
+      wp_apply (acquire_spec); eauto.
+      iDestruct 1 as (n1 n2) "(Hr & Hγ1● & Hγ2●)".
+      iDestruct (ghost_var_agree with "Hγ2● Hγ2◯") as %->.
+      destruct n1.
+      + wp_seq. wp_load. wp_op. wp_store.
+        iMod (ghost_var_update γ2 false with "Hγ2● Hγ2◯") as "[Hγ2● Hγ2◯]".
+        wp_apply (release_spec with "[Hr Hγ1● Hγ2●]"); auto.
+        iSplit; eauto.
+        iExists _, _. iFrame.
+      + wp_seq. wp_load. wp_op. wp_store.
+        iMod (ghost_var_update γ2 false with "Hγ2● Hγ2◯") as "[Hγ2● Hγ2◯]".
+        wp_apply (release_spec with "[Hr Hγ1● Hγ2●]"); auto.
+        iSplit; eauto.
+        iExists _, _. iFrame.
+    - (* exercise *)
+      iIntros (v1 v2) "OWN".
+      iNext.
+      wp_seq.
+      wp_apply (acquire_spec with "Hl"). iDestruct 1 as (n1 n2) "(Hr & Hγ1● & Hγ2●)".
+      iDestruct "OWN" as "[Hγ1◯ Hγ2◯]".
+      iDestruct (ghost_var_agree with "Hγ1● Hγ1◯") as %->.
+      iDestruct (ghost_var_agree with "Hγ2● Hγ2◯") as %->.
+      iDestruct "Hr" as "[A|B]".
+      + wp_exec.
+        iApply "Post".
+        eauto.
+      + wp_exec.
+        iApply "Post".
+        eauto.
+  Qed.
+
 End proof.
